forward: start to strengthen invariant
We attempted to allow for units in the candidates for forward
subsumption, but this turned to be too complicated. So we started to
strengthen the invariants, requiring various changing in the
strengthening algorithm. For example, we want to ensure that the
candidate clause is not in the occurence lists and has not been deleted.

Weidenbach_Book/IsaSAT/IsaSAT_Simplify_Forward_Subsumption.thy
@@ -144,8 +144,8 @@ definition forward_subsumption_one_wl2_rel where
      changed = changed' \<and> set_mset (all_init_atms_st S) = set_mset (all_init_atms_st S\<^sub>0) \<and>
       (changed \<longrightarrow> (D', {#}) \<in> clause_hash_ref (all_init_atms_st S)) \<and>
       (\<not>changed \<longrightarrow> D' = D \<and> occs' = occs \<and> get_clauses_wl S \<propto> C = get_clauses_wl S\<^sub>0 \<propto> C) \<and>
-      correct_occurence_list S occs' (if changed then size (get_clauses_wl S\<^sub>0 \<propto> C) else n) \<and>
-     all_occurrences (all_init_atms_st S) occs' \<subseteq># add_mset C (all_occurrences  (all_init_atms_st S) occs) \<and>
+        correct_occurence_list S occs' (if changed then size (get_clauses_wl S\<^sub>0 \<propto> C) else n) \<and>
+        all_occurrences (all_init_atms_st S) occs' \<subseteq># add_mset C (all_occurrences  (all_init_atms_st S) occs) \<and>
      (S,T)\<in>Id
     }\<close>
 
@@ -515,16 +515,18 @@ definition try_to_forward_subsume_wl2 :: \<open>nat \<Rightarrow> occurences \<R
   RETURN (occs, D, S)
   }\<close>
 
-lemma
+lemma try_to_forward_subsume_wl2_try_to_forward_subsume_wl:
   assumes \<open>(C, E) \<in> nat_rel\<close> and
-    DG: \<open>(D, G) \<in> clause_hash_ref (all_init_atms_st S\<^sub>0)\<close> and
-    G: \<open>G = mset (get_clauses_wl S\<^sub>0 \<propto> C)\<close> and
+    DG: \<open>(D, G) \<in> clause_hash_ref (all_init_atms_st T\<^sub>0)\<close> and
+    G: \<open>G = mset (get_clauses_wl T\<^sub>0 \<propto> C)\<close> and
     occs: \<open>correct_occurence_list S\<^sub>0 occs n\<close> and
-    n: \<open>n\<le> size (get_clauses_wl S\<^sub>0 \<propto> C)\<close> and
-    C_occs: \<open>C \<notin># all_occurrences (all_init_atms_st S\<^sub>0) occs\<close> and
+    n: \<open>n\<le> length (get_clauses_wl S\<^sub>0 \<propto> C)\<close> and
+    C_occs: \<open>C \<notin># all_occurrences (all_init_atms_st T\<^sub>0) occs\<close> and
     \<open>(S\<^sub>0, T\<^sub>0) \<in> Id\<close>
   shows \<open>try_to_forward_subsume_wl2 C occs D S\<^sub>0 \<le>
-    \<Down>{((occs', D', T), U). (T, U) \<in> Id \<and> (D', {#}) \<in> clause_hash_ref (all_init_atms_st T)}
+    \<Down>{((occs', D', T), U). (T, U) \<in> Id \<and> (D', {#}) \<in> clause_hash_ref (all_init_atms_st T) \<and>
+       correct_occurence_list U occs' (max (length (get_clauses_wl S\<^sub>0 \<propto> C)) n) \<and>
+       all_occurrences (all_init_atms_st U) occs' \<subseteq># add_mset C (all_occurrences  (all_init_atms_st S\<^sub>0) occs)}
     (try_to_forward_subsume_wl E T\<^sub>0)\<close>
 proof -
   have eq: \<open>T\<^sub>0 = S\<^sub>0\<close> \<open>E = C\<close>
@@ -556,8 +558,10 @@ proof -
       (\<not>changed \<longrightarrow> (D', mset (get_clauses_wl U \<propto> C)) \<in> clause_hash_ref (all_init_atms_st U)) \<and> 
       (changed \<longrightarrow> ebreak \<and> (D', {#}) \<in> clause_hash_ref (all_init_atms_st U)) \<and> 
     (ebreak, ebreak') \<in> bool_rel \<and>
-    (\<not>changed \<longrightarrow> correct_occurence_list U occs' n \<and> occs' = occs \<and> get_clauses_wl U \<propto> C = get_clauses_wl S\<^sub>0 \<propto> C) \<and>
-    (changed \<longrightarrow> correct_occurence_list U occs' (max (length (get_clauses_wl S\<^sub>0 \<propto> C)) n)) \<and>
+    (\<not>changed \<longrightarrow> correct_occurence_list U occs' n \<and> occs' = occs \<and> get_clauses_wl U \<propto> C = get_clauses_wl S\<^sub>0 \<propto> C \<and>
+        all_occurrences (all_init_atms_st V) occs' = all_occurrences  (all_init_atms_st S\<^sub>0) occs) \<and>
+    (changed \<longrightarrow> correct_occurence_list U occs' (max (length (get_clauses_wl S\<^sub>0 \<propto> C)) n) \<and>
+       all_occurrences (all_init_atms_st V) occs' \<subseteq># add_mset C (all_occurrences  (all_init_atms_st S\<^sub>0) occs)) \<and>
     U = V}\<close> (is \<open>_ \<Longrightarrow> _ \<in> ?R\<close>)
     for ebreak ebreaka
     using assms by auto
@@ -622,58 +626,196 @@ proof -
     subgoal using DG G by (auto dest: clause_hash_ref_cong[OF try_to_forward_subsume_wl2_invD])
     subgoal by auto
     subgoal using n by auto
-    subgoal using C_occs by (auto dest: all_occurrences_cong[OF try_to_forward_subsume_wl2_invD])
+    subgoal using C_occs by (auto dest: all_occurrences_cong[OF try_to_forward_subsume_wl2_invD] simp: eq)
     subgoal for a ebreak ebreaka x x' x1 x2 x1a x2a x1b x2b x1c x2c x1d x2d x1e x2e x1f x2f
       using K[of x1 x2a] by auto
     subgoal by auto
-    subgoal
-      by (auto 4 3 dest: clause_hash_ref_cong
-        simp add: correct_occurence_list_size_mono[of _ _ _ \<open>(max (length (get_clauses_wl S\<^sub>0 \<propto> C)) n)\<close>]
-        forward_subsumption_one_wl2_rel_def)
+    subgoal for na ebreak ebreaka x x' x1 x2 x1a x2a x1b x2b x1c x2c x1d x2d x1e x2e x1f x2f uu_ xa x'a x1g x2g x1h x2h x1i x2i
+      x1j x2j ebreakb ebreakc
+      apply (frule all_occurrences_cong[OF try_to_forward_subsume_wl2_invD])
+      apply (clarsimp simp add: forward_subsumption_one_wl2_rel_def)
+      apply (auto dest: 
+        intro: correct_occurence_list_size_mono[of _ _ _ \<open>(max (length (get_clauses_wl S\<^sub>0 \<propto> C)) n)\<close>]
+        simp: clause_hash_ref_cong[of \<open>all_init_atms_st x1g\<close>]
+        all_occurrences_cong[of \<open>all_init_atms_st x1g\<close> \<open>all_init_atms_st x2a\<close>]
+        forward_subsumption_one_wl2_rel_def
+        simp: )
+     done
     apply (rule mop_ch_remove_all2; assumption)
     subgoal by auto
     subgoal for na ebreak ebreaka x x' x1 x2 x1a x2a x1b x2b x1c x2c x1d x2d x1e x2e x1f x2f
-      by auto
+      using n by (auto simp: eq intro: correct_occurence_list_size_mono)
     done
 qed
 
 
-definition forward_subsumption_all_wl2_inv :: \<open>nat twl_st_wl \<Rightarrow> nat list \<Rightarrow> nat \<times> _ \<times> _ \<times> nat twl_st_wl \<Rightarrow> bool\<close> where
-  \<open>forward_subsumption_all_wl2_inv = (\<lambda>S xs (i, occs, D, s).
+definition forward_subsumption_all_wl2_inv :: \<open>nat twl_st_wl \<Rightarrow> nat list \<Rightarrow> nat \<times> _ \<times> _ \<times> nat twl_st_wl \<times> nat \<Rightarrow> bool\<close> where
+  \<open>forward_subsumption_all_wl2_inv = (\<lambda>S xs (i, occs, D, s, n).
   (D, {#}) \<in> clause_hash_ref (all_init_atms_st s) \<and>
   forward_subsumption_all_wl_inv S (mset (drop i xs), s))
   \<close>
 
+(*TODO populate occs*)
+
+definition populate_occs_inv where
+  \<open>populate_occs_inv S xs = (\<lambda>(i, occs, cands).
+  all_occurrences (all_init_atms_st S) occs + mset cands \<subseteq># mset (take i xs) \<and>
+  mset xs \<subseteq># dom_m (get_clauses_wl S) \<and>
+  distinct cands \<and>
+  correct_occurence_list S occs 2)\<close>
+
+
+definition populate_occs_spec where
+  \<open>populate_occs_spec S = (\<lambda>(occs, cands).
+  all_occurrences (all_init_atms_st S) occs + mset cands \<subseteq># dom_m (get_clauses_wl S) \<and>
+  distinct cands \<and> sorted_wrt (\<lambda>a b. length (get_clauses_wl S \<propto> a) \<le> length (get_clauses_wl S \<propto> b)) cands \<and>
+  correct_occurence_list S occs 2 \<and>
+  (\<forall>C\<in># dom_m (get_clauses_wl S). \<forall>L\<in> set (get_clauses_wl S \<propto> C). undefined_lit (get_trail_wl S) L))\<close>
+
+definition populate_occs :: \<open>nat twl_st_wl \<Rightarrow> _ nres\<close> where
+  \<open>populate_occs S = do {
+    xs \<leftarrow> SPEC (\<lambda>xs. mset xs \<subseteq># dom_m (get_clauses_wl S));
+    let n = size xs;
+    occs \<leftarrow> mop_occ_list_create (set_mset (all_init_atms_st S));
+    let cands = [];
+    (xs, occs, cands) \<leftarrow> WHILE\<^sub>T\<^bsup>populate_occs_inv S xs\<^esup> (\<lambda>(i, occs, cands). i < n)
+    (\<lambda>(i, occs, cands). do {
+      let C = xs ! i;
+      if C \<in># dom_m (get_clauses_wl S) \<and> length (get_clauses_wl S \<propto> C) = 2 then do {
+        occs \<leftarrow> push_to_occs_list2 C S occs;
+        RETURN (i+1, occs, cands)
+      }
+      else  do {
+        cand \<leftarrow> SPEC (\<lambda>b. b \<longrightarrow> C \<in># dom_m (get_clauses_wl S) \<and> length (get_clauses_wl S \<propto> C) > 2);
+        if cand then RETURN (i+1, occs, cands @ [C])
+        else RETURN (i+1, occs, cands)
+        }
+      }
+      )
+      (0, occs, cands);
+     cands \<leftarrow> SPEC (\<lambda>cands'. mset cands' = mset cands \<and> sorted_wrt (\<lambda>a b. length (get_clauses_wl S \<propto> a) \<le> length (get_clauses_wl S \<propto> b)) cands');
+     RETURN (occs, cands)
+  }\<close>
+
+lemma \<open>populate_occs S \<le> SPEC(populate_occs_spec S)\<close>
+  sorry
 definition forward_subsumption_all_wl2 :: \<open>nat twl_st_wl \<Rightarrow> _ nres\<close> where
   \<open>forward_subsumption_all_wl2 = (\<lambda>S. do {
   ASSERT (forward_subsumption_all_wl_pre S);
-  xs \<leftarrow> SPEC (\<lambda>xs. mset xs \<subseteq># dom_m (get_clauses_wl S) \<and> sorted_wrt (\<lambda>a b. length (get_clauses_wl S \<propto> a) \<le> length (get_clauses_wl S \<propto> b)) xs);
-  occs \<leftarrow> mop_occ_list_create (set_mset (all_init_atms_st S));
-  let n = length xs;
+  (occs, xs) \<leftarrow> SPEC (populate_occs_spec S);
+  let m = length xs;
   D \<leftarrow> mop_ch_create (set_mset (all_init_atms_st S));
-  (xs, occs, D, S) \<leftarrow>
-    WHILE\<^sub>T\<^bsup> forward_subsumption_all_wl2_inv S xs \<^esup> (\<lambda>(i, occs, D, S). i < n \<and> get_conflict_wl S = None)
-    (\<lambda>(i, occs, D, S). do {
+  (xs, occs, D, S, _) \<leftarrow>
+    WHILE\<^sub>T\<^bsup> forward_subsumption_all_wl2_inv S xs \<^esup> (\<lambda>(i, occs, D, S, n). i < m \<and> get_conflict_wl S = None)
+    (\<lambda>(i, occs, D, S, n). do {
        let C = xs!i;
        if C \<notin># dom_m (get_clauses_wl S)
-       then RETURN (i+1, occs, D, S)
+       then RETURN (i+1, occs, D, S, n)
        else do {
-         S \<leftarrow> simplify_clause_with_unit_st_wl C  S;
-         if get_conflict_wl S = None \<and> C \<in># dom_m (get_clauses_wl S) \<and> length (get_clauses_wl S \<propto> C) > 2 then do {
-           D \<leftarrow> mop_ch_add_all (mset (get_clauses_wl S \<propto> C)) D;
-           (occs, D, S) \<leftarrow> try_to_forward_subsume_wl2 C occs D S;
-           RETURN (i+1, occs, D, S)
+         T \<leftarrow> simplify_clause_with_unit_st_wl C S;
+         ASSERT (set_mset (all_init_atms_st S) = set_mset (all_init_atms_st T));
+         ASSERT (get_trail_wl T = get_trail_wl S);
+         ASSERT (\<forall>D \<in># dom_m (get_clauses_wl T). (D \<noteq> C \<longrightarrow> get_clauses_wl T \<propto> D = get_clauses_wl S \<propto> D));
+         ASSERT (C \<in># dom_m (get_clauses_wl T) \<longrightarrow> (\<forall>L\<in>set (get_clauses_wl T \<propto> C). undefined_lit (get_trail_wl T) L));
+         if get_conflict_wl T = None \<and> C \<in># dom_m (get_clauses_wl T) \<and> length (get_clauses_wl T \<propto> C) > 2 then do {
+           D \<leftarrow> mop_ch_add_all (mset (get_clauses_wl T \<propto> C)) D;
+           (occs, D, T) \<leftarrow> try_to_forward_subsume_wl2 C occs D T;
+           RETURN (i+1, occs, D, T, max (length (get_clauses_wl T \<propto> C)) n)
          }
-         else RETURN (i+1, occs, D, S)
+         else RETURN (i+1, occs, D, T, n)
       }
     })
-    (0, occs, D, S);
+    (0, occs, D, S, 2);
   RETURN S
   }
 )\<close>
+thm forward_subsumption_one_wl_def
+thm forward_subsumption_one_wl_pre_def
+thm forward_subsumption_one_wl_pre_def 
+thm forward_subsumption_one_wl_select_def
+lemma
+  \<open>forward_subsumption_all_wl2 S \<le> \<Down>Id (forward_subsumption_all_wl S)\<close>
+proof -
+  have forward_subsumption_all_wl_alt_def:
+    \<open>forward_subsumption_all_wl = (\<lambda>S. do {
+  ASSERT (forward_subsumption_all_wl_pre S);
+    xs \<leftarrow> SPEC (\<lambda>xs. xs \<subseteq># dom_m (get_clauses_wl S));
+  let _ = size xs;
+   D \<leftarrow> RETURN ({#} :: nat clause);
+  ASSERT (D = {#});
+  (xs, S) \<leftarrow>
+    WHILE\<^sub>T\<^bsup> forward_subsumption_all_wl_inv S \<^esup> (\<lambda>(xs, S). xs \<noteq> {#} \<and> get_conflict_wl S = None)
+    (\<lambda>(xs, S). do {
+       C \<leftarrow> SPEC (\<lambda>C. C \<in># xs);
+       if C \<notin># dom_m (get_clauses_wl S)
+       then RETURN (remove1_mset C xs, S)
+       else do {
+         S \<leftarrow> simplify_clause_with_unit_st_wl C S;
+         if get_conflict_wl S = None \<and> C \<in># dom_m (get_clauses_wl S) \<and> length (get_clauses_wl S \<propto> C) > 2 then do {
+           let _ = mset (get_clauses_wl S \<propto> C) + {#};
+           (S) \<leftarrow> try_to_forward_subsume_wl C S;
+           RETURN (remove1_mset C xs, S)
+         }
+         else RETURN (remove1_mset C xs, S)
+      }
+    })
+    (xs, S);
+  RETURN S
+  }
+           )\<close>
+    unfolding forward_subsumption_all_wl_def Let_def by auto
+  have [refine]: \<open>SPEC
+  (\<lambda>xs. mset xs \<subseteq># dom_m (get_clauses_wl S) \<and>
+     sorted_wrt (\<lambda>a b. length (get_clauses_wl S \<propto> a) \<le> length (get_clauses_wl S \<propto> b)) xs)
+    \<le> \<Down> {(xs,ys). mset xs = ys \<and> mset xs \<subseteq># dom_m (get_clauses_wl S) \<and>
+     sorted_wrt (\<lambda>a b. length (get_clauses_wl S \<propto> a) \<le> length (get_clauses_wl S \<propto> b)) xs}
+    (SPEC (\<lambda>xs. xs \<subseteq># dom_m (get_clauses_wl S)))\<close>
+    by (auto intro!: RES_refine)
+  have [refine]: \<open>SPEC (populate_occs_spec S) \<le> \<Down> {((occs,xs), ys).  ys = mset xs \<and> populate_occs_spec S (occs, xs)}(SPEC (\<lambda>xs. xs \<subseteq># dom_m (get_clauses_wl S)))\<close>
+    (is \<open>_ \<le> \<Down> ?populate _\<close>)
+    unfolding populate_occs_spec_def prod.simps
+    by (rule RES_refine)
+     (auto dest: mset_le_decr_left2)
+  have loop_init: \<open>(occsxs, xsa) \<in> ?populate \<Longrightarrow>
+    occsxs = (occs, xs) \<Longrightarrow>
+    (D, D') \<in> clause_hash_ref (all_init_atms_st S) \<Longrightarrow>
+    D' = {#} \<Longrightarrow>
+    forward_subsumption_all_wl_inv S (xsa, S) \<Longrightarrow> ((0, occs, D, S, 2), xsa, S) \<in>
+    {((i, occs', D, U, n), (xsa, V)). (U,V)\<in>Id \<and> i \<le> length xs \<and>
+    (D, {#}) \<in> clause_hash_ref (all_init_atms_st V) \<and>
+    correct_occurence_list U occs n \<and> xsa = mset (drop i xs)}\<close> 
+    (is \<open>_ \<Longrightarrow> _ \<Longrightarrow> _ \<Longrightarrow>_ \<Longrightarrow> _ \<Longrightarrow> _ \<in> ?loopinv\<close>) for D occs xsa aa xs occsxs uu D'
+    by (auto simp: populate_occs_spec_def)
+  have [refine]: \<open>(a,b) \<in> Id \<Longrightarrow> (c, d) \<in> Id \<Longrightarrow> simplify_clause_with_unit_st_wl a c \<le>\<Down>Id (simplify_clause_with_unit_st_wl b d)\<close> for a b c d
+    by auto
+      find_theorems simplify_clause_with_unit_st_wl
+  show ?thesis
+    unfolding forward_subsumption_all_wl_alt_def forward_subsumption_all_wl2_def
+    apply (rewrite at \<open>let _ = length _ in _\<close> Let_def)
+    apply (refine_vcg mop_occ_list_create mop_ch_create mop_ch_add_all
+      try_to_forward_subsume_wl2_try_to_forward_subsume_wl)
+    apply (rule loop_init; assumption)
+    subgoal unfolding forward_subsumption_all_wl2_inv_def by auto
+    subgoal by auto
+    subgoal by (auto simp: in_set_dropI)
+    subgoal by auto
+    subgoal by (auto simp: drop_Suc_nth)
+    subgoal by auto
+    subgoal sorry
+    subgoal by auto
+    apply (solves auto)
+    subgoal sorry
+    subgoal by auto
+    subgoal by auto
+    apply (subst clause_hash_ref_cong)
+    defer apply assumption
+    subgoal by auto
+    subgoal
+thm mop_ch_add_all
+  thm correct_occurence_list_def
+    apply assumption
 
-
-  find_theorems drop Suc nth
+  find_theorems mop_ch_create
 thm subsume_clauses_match_def
 thm forward_subsumption_one_wl_def
 thm try_to_forward_subsume_wl_def
